spec/design/X64/Arch_Structs_B.thy
@@ -19,6 +19,11 @@ begin
 
 context Arch begin global_naming X64_H
 
+datatype x64_vspace_region_use =
+     X64VSpaceUserRegion
+   | X64VSpaceInvalidRegion
+   | X64VSpaceKernelWindow
+   | X64VSpaceDeviceWindow
 
 end (* context X64 *)
 
